src/Common/i2list2.v
@@ -1,7 +1,7 @@
 Generalizable All Variables.
 Set Implicit Arguments.
 
-Require Import Coq.Lists.List Coq.Strings.String Coq.Arith.Arith ADTSynthesis.Common.ilist.
+Require Import Coq.Lists.List Coq.Strings.String Coq.Arith.Arith ADTSynthesis.Common.ilist ADTSynthesis.Common.ilist2.
 
 Section i2list2.
 
@@ -15,19 +15,19 @@ Section i2list2.
   Variable B : A -> Type. (* The type of indexed elements. *)
   Variable C : forall a, B a ->  Type. (* The type of doubly-indexed elements. *)
 
-  Inductive i2list2 : forall (As : list A), ilist B As -> Type :=
-  | i2cons2 : forall a As (Bs : ilist B (a :: As))
-                    (c : C (ilist_hd Bs)),
-               i2list2 (ilist_tl Bs) -> i2list2 Bs
-  | i2nil2 : forall Bs : ilist B nil, i2list2 Bs.
+  Inductive i2list2 : forall (As : list A), ilist2 B As -> Type :=
+  | i2cons2 : forall a As (Bs : ilist2 B (a :: As))
+                    (c : C (ilist2_hd Bs)),
+               i2list2 (ilist2_tl Bs) -> i2list2 Bs
+  | i2nil2 : forall Bs : ilist2 B nil, i2list2 Bs.
 
   (* Get the car of an i2list2. *)
 
   Definition i2list2_hd (As : list A)
-             (Bs : ilist B As)
+             (Bs : ilist2 B As)
              (i2l : i2list2 Bs) :
-    match As return forall Bs : ilist B As, i2list2 Bs -> Type with
-      | a :: As' => fun Bs i2l => C (ilist_hd Bs)
+    match As return forall Bs : ilist2 B As, i2list2 Bs -> Type with
+      | a :: As' => fun Bs i2l => C (ilist2_hd Bs)
       | nil => fun _ _ => unit
     end Bs i2l :=
     match i2l with
@@ -37,11 +37,11 @@ Section i2list2.
 
   (* Get the cdr of an i2list2. *)
   Definition i2list2_tl (As : list A)
-             (Bs : ilist B As)
+             (Bs : ilist2 B As)
              (i2l : i2list2 Bs) :
     match As as As' return
-          forall Bs : ilist B As', i2list2 Bs -> Type with
-      | a :: As' => fun Bs il => i2list2 (ilist_tl Bs)
+          forall Bs : ilist2 B As', i2list2 Bs -> Type with
+      | a :: As' => fun Bs il => i2list2 (ilist2_tl Bs)
       | nil => fun _ _ => unit
     end Bs i2l :=
     match i2l with
@@ -51,93 +51,13 @@ Section i2list2.
 
   (* Membership in a doubly-indexed list. *)
   Inductive i2list2_In
-  : forall {a : A} {b : B a} (c : C b) (As : list A) (il : ilist B As) (i2l : i2list2 il), Prop :=
-  | In2_hd : forall a' As (Bs : ilist B (a' :: As)) (i2l : i2list2 (ilist_tl Bs)) c,
+  : forall {a : A} {b : B a} (c : C b) (As : list A) (il : ilist2 B As) (i2l : i2list2 il), Prop :=
+  | In2_hd : forall a' As (Bs : ilist2 B (a' :: As)) (i2l : i2list2 (ilist2_tl Bs)) c,
               i2list2_In c (i2cons2 Bs c i2l)
-  | In2_tl : forall a a' As (Bs : ilist B (a' :: As)) (b' : B a) c' (i2l : i2list2 (ilist_tl Bs)) (c : C b'),
+  | In2_tl : forall a a' As (Bs : ilist2 B (a' :: As)) (b' : B a) c' (i2l : i2list2 (ilist2_tl Bs)) (c : C b'),
               i2list2_In c i2l ->
               i2list2_In c (i2cons2 Bs c' i2l).
 
-  (* Fixpoint siglist2i2list2 *)
-  (*          (As : list A) *)
-  (*          (il : ilist (fun a => sigT (@C a)) As) *)
-  (* : i2list2 (imap _ (fun a => @projT1 _ (@C a)) il)  := *)
-  (*   match il *)
-  (*         return i2list2 (imap _ (fun a => @projT1 _ (@C a)) il) *)
-  (*   with *)
-  (*     | inil => i2nil2 *)
-  (*     | icons a As' (existT b c) il' => i2cons2 c (siglist2i2list2 il') *)
-  (*   end. *)
-
-  (* (* and vice versa. *) *)
-  (* Fixpoint i2list22siglist {As : list A} {Bs : ilist B As} *)
-  (* (i2l : i2list2 Bs) *)
-  (* : ilist (fun a => sigT (@C a)) As := *)
-  (*   match i2l in @i2list2 As' Bs' return ilist (fun a => sigT (@C a)) As' with *)
-  (*     | i2nil2 => @inil _ _ *)
-  (*     | i2cons2 a As b Bs' c Cs' => *)
-  (*       icons a (existT _ b c) (i2list22siglist Cs') *)
-  (*   end. *)
-
-  (* (* i2list22siglist is the inverse of siglist2i2list2 *) *)
-  (* Lemma siglist2i2list2_id *)
-  (* : forall As (Bs : ilist _ As), *)
-  (*     i2list22siglist (siglist2i2list2 Bs) = Bs. *)
-  (* Proof. *)
-  (*   induction Bs; simpl; auto. *)
-  (*   destruct b; simpl; congruence. *)
-  (* Qed. *)
-
-  (* and vice-versa.
-
-  (* i2list22siglist is the inverse of siglist2i2list2 *)
-  Lemma i2list22siglist_id
-  : forall As Bs (Cs : i2list2 Bs),
-      siglist2i2list2 (i2list22siglist Cs) = Cs.
-  Proof.
-    induction Bs; simpl; auto.
-    destruct b; simpl; congruence.
-  Qed.
-
-  Fixpoint ilist2siglist_map
-          As (il : ilist As)
-  : map (@projT1 _ B) (ilist2siglist il) = As :=
-    match il as il' in ilist As' return
-          map (@projT1 _ B) (ilist2siglist il') = As' with
-      | inil => eq_refl
-      | icons a As' b il' => f_equal (fun b' => cons a b') (ilist2siglist_map il')
-    end.
-
-  Lemma ilist2sislist_map_cons
-  : forall a b As (il il' : ilist As),
-      match ilist2siglist_map il in (_ = y) return (ilist y -> Prop) with
-        | eq_refl =>
-          fun il' => siglist2ilist (ilist2siglist il) = il'
-      end il'
-      ->
-      match
-        f_equal (fun b' : list A => a :: b') (ilist2siglist_map il) in (_ = y)
-        return (ilist y -> Prop)
-      with
-        | eq_refl =>
-          fun il' : ilist (a :: map (projT1 (P:=B)) (ilist2siglist il)) =>
-            icons b (siglist2ilist (ilist2siglist il)) = il'
-      end (icons b il').
-  Proof.
-    intros until il; destruct (ilist2siglist_map il); congruence.
-  Qed.
-
-  Lemma ilist2siglist_id
-  : forall As (il : ilist As),
-      match (ilist2siglist_map il) in (_ = y) return
-            forall (il' : ilist y), Prop
-      with
-        | eq_refl => fun il' => siglist2ilist (ilist2siglist il) = il'
-      end il.
-  Proof.
-    induction il; simpl; auto.
-    apply ilist2sislist_map_cons; auto.
-  Qed. *)
 
   (* Looking up the ith value, returning None for indices not in the list *)
 
@@ -145,53 +65,53 @@ Section i2list2.
 
   Fixpoint i2th_error2
           (As : list A)
-          (Bs : ilist B As)
+          (Bs : ilist2 B As)
           (i2l : i2list2 Bs)
           (n : nat)
           {struct n}
-  : Dep_Option_elim_P C (ith_error Bs n) :=
+  : Dep_Option_elim_P C (ith2_error Bs n) :=
     match n as n' return
-          forall (Bs : ilist B As),
+          forall (Bs : ilist2 B As),
             i2list2 Bs
-            -> Dep_Option_elim_P C (ith_error Bs n')
+            -> Dep_Option_elim_P C (ith2_error Bs n')
     with
       | 0 => fun Bs =>
                match Bs as Bs' return
                      i2list2 Bs'
-                     -> Dep_Option_elim_P C (ith_error Bs' 0) with
-                 | inil => fun i2l => I
-                 | icons a As' b Bs' => fun i2l => i2list2_hd i2l
+                     -> Dep_Option_elim_P C (ith2_error Bs' 0) with
+                 | inil2 => fun i2l => I
+                 | icons2 a As' b Bs' => fun i2l => i2list2_hd i2l
                end
       | S n => fun Bs =>
                  match Bs as Bs' return
                        i2list2 Bs'
-                       -> Dep_Option_elim_P C (ith_error Bs' (S n)) with
-                   | inil => fun i2l => I
-                   | icons a As' b Bs' => fun i2l => i2th_error2 (i2list2_tl i2l) n
+                       -> Dep_Option_elim_P C (ith2_error Bs' (S n)) with
+                   | inil2 => fun i2l => I
+                   | icons2 a As' b Bs' => fun i2l => i2th_error2 (i2list2_tl i2l) n
                  end
     end Bs i2l.
 
   Fixpoint i2th_error2'
           (As : list A)
-          (Bs : ilist B As)
+          (Bs : ilist2 B As)
           (i2l : i2list2 Bs)
           (n : nat)
           {struct n}
-  : Dep_Option_elim_P C (ith_error Bs n) :=
+  : Dep_Option_elim_P C (ith2_error Bs n) :=
     match n as n' return
-          forall (Bs : ilist B As),
+          forall (Bs : ilist2 B As),
             i2list2 Bs
-            -> Dep_Option_elim_P C (ith_error Bs n')
+            -> Dep_Option_elim_P C (ith2_error Bs n')
     with
       | 0 => fun Bs i2l =>
                match i2l as i2l' in i2list2 Bs' return
-                     Dep_Option_elim_P C (ith_error Bs' 0) with
+                     Dep_Option_elim_P C (ith2_error Bs' 0) with
                  | i2nil2 _ => I
                  | i2cons2 a As' Bs' c i2l' => c
                end
       | S n => fun Bs i2l =>
                  match i2l as i2l' in i2list2 Bs' return
-                       Dep_Option_elim_P C (ith_error Bs' (S n)) with
+                       Dep_Option_elim_P C (ith2_error Bs' (S n)) with
                    | i2nil2 _ => I
                    | i2cons2 a As' Bs' c i2l' => i2th_error2' i2l' n
                  end
@@ -204,39 +124,39 @@ Section i2list2.
           (default_B : B default_A)
           (default_C : C default_B)
           (As : list A)
-          (Bs : ilist B As)
+          (Bs : ilist2 B As)
           (i2l : i2list2 Bs)
           (n : nat)
           {struct As}
-  : C (ith_default default_A default_B Bs n) :=
+  : C (ith2_default default_A default_B Bs n) :=
     match As as As', n as n' return
-          forall (Bs' : ilist B As'),
+          forall (Bs' : ilist2 B As'),
             i2list2 Bs'
-            -> C (ith_default default_A default_B Bs' n') with
+            -> C (ith2_default default_A default_B Bs' n') with
       | a :: As', 0    => @i2list2_hd (a :: As')
       | a :: As', S n' => fun il i2l => i2th_default2 default_C (i2list2_tl i2l) n'
       | nil      , 0    => fun il i2l => default_C
       | nil      , S n' => fun il i2l => default_C
     end Bs i2l.
 
-  Lemma i2list2_invert (As : list A) (Bs : ilist B As) (Cs : i2list2 Bs):
+  Lemma i2list2_invert (As : list A) (Bs : ilist2 B As) (Cs : i2list2 Bs):
     match Bs as Bs' return i2list2 Bs' -> Prop with
-      | icons a As b Bs' => fun Cs =>
+      | icons2 a As b Bs' => fun Cs =>
                            exists (c : C b) (Cs' : i2list2 Bs'),
-                             Cs = i2cons2 (icons a b Bs') c Cs'
-      | inil => fun Cs => Cs = i2nil2 (inil _)
+                             Cs = i2cons2 (icons2 a b Bs') c Cs'
+      | inil2 => fun Cs => Cs = i2nil2 (inil2 _)
     end Cs.
   Proof.
     destruct Cs.
-    - destruct (ilist_invert Bs) as [b [Bs' Bs'_eq]]; subst.
+    - destruct (ilist2_invert Bs) as [b [Bs' Bs'_eq]]; subst.
       eexists; eauto.
-    - pose (ilist_invert Bs) as Bs_eq; simpl in Bs_eq; subst; eauto.
+    - pose (ilist2_invert Bs) as Bs_eq; simpl in Bs_eq; subst; eauto.
   Qed.
 
   Lemma i2th_default2_In :
     forall (n : nat)
            (As : list A)
-           (Bs : ilist B As)
+           (Bs : ilist2 B As)
            (Cs : i2list2 Bs)
            (default_A : A)
            (default_B : B default_A)
@@ -244,16 +164,16 @@ Section i2list2.
       n < List.length As ->
       i2list2_In (i2th_default2 default_C Cs n) Cs.
   Proof.
-    ith_induction n As; simpl;
+    ith2_induction n As; simpl;
     destruct (i2list2_invert Cs) as [c [Cs' Cs_eq]]; subst; simpl;
-    [apply (In2_hd (icons a b il) Cs' c) |  constructor 2];
+    [apply (In2_hd (icons2 a b il) Cs' c) |  constructor 2];
     eauto with arith.
   Qed.
 
   Lemma i2th_default2_indep :
     forall (n : nat)
            (As : list A)
-           (Bs : ilist B As)
+           (Bs : ilist2 B As)
            (Cs : i2list2 Bs)
            (default_A : A)
            (default_B : B default_A)
@@ -266,236 +186,6 @@ Section i2list2.
 
 End i2list2.
 
-(** ** Mapping a function over a(n i)[list], in two non-dependent ways
-Section i2list2_map.
-  Context {A} (B : A -> Type).
-
-  Fixpoint imap_list (f : forall a : A, B a) (As : list A) : ilist B As
-    := match As with
-         | nil => inil _
-         | x::xs => @icons _ B x _ (f x) (imap_list f xs)
-       end.
-
-  Fixpoint map_ilist {C} (f : forall (a : A), B a -> C) {As} (Bs : ilist B As) : list C
-    := match Bs with
-         | inil => nil
-         | icons _ _ x xs => (f _ x)::map_ilist f xs
-       end.
-
-End ilist_map.
-
-Section of_list.
-  Context {T : Type}.
-
-  Definition ilist_of_list : forall ls : list T, ilist (fun _ => T) ls := imap_list (fun _ => T) (fun x => x).
-  Definition list_of_ilist {T'} {is} (ls : ilist (fun _ : T' => T) is) : list T
-    := map_ilist (B := fun _ => T) (fun _ x => x) ls.
-
-  Lemma list_of_ilist_of_list ls : list_of_ilist (ilist_of_list ls) = ls.
-  Proof.
-    unfold list_of_ilist, ilist_of_list.
-    induction ls; simpl in *; f_equal; assumption.
-  Qed.
-End of_list.
-
-
-Section ilist_imap.
-
-  (* Mapping a function over an indexed list. *)
-
-  Variable A : Type. (* The indexing type. *)
-  Variable B B' : A -> Type. (* The two types of indexed elements. *)
-  Variable f : forall a, B a -> B' a. (* The function to map over the list. *)
-
-  Fixpoint imap (As : list A)
-           (il : ilist B As)
-  : ilist B' As :=
-    match il in ilist _ As return ilist _ As with
-      | icons a As b il' => icons a (f b) (imap il')
-      | inil => inil B'
-    end.
-
-  (* [imap] behaves as expected with the [ith_default] lookup
-     function. *)
-  Lemma ith_default_imap :
-    forall (n : nat)
-           (As : list A)
-           (il : ilist _ As)
-           (default_A : A)
-           (default_B : B default_A),
-      f (ith_default default_A default_B il n) =
-      ith_default default_A (f default_B) (imap il) n.
-  Proof.
-    induction n; destruct As; simpl; eauto;
-    intros; icons_invert; simpl; auto.
-  Qed.
-
-  (* Mapping [f] over a dependent option. *)
-  Definition Dep_Option_Map
-             (a_opt : option A)
-             (b_opt : Dep_Option B a_opt) :
-    Dep_Option B' a_opt :=
-    match b_opt with
-      | Dep_Some a b' => Dep_Some B' a (f b')
-      | Dep_None => Dep_None B'
-    end.
-
-  (* Applying [f] to the value projected from a dependent option [b_opt]
-     is the same as mapping [f] over the [b_opt] and projecting.
-   *)
-  Lemma Dep_Option_Map_elim
-  : forall (a_opt : option A)
-           (b_opt : Dep_Option B a_opt),
-      Dep_Option_elim (Dep_Option_Map b_opt) =
-      match a_opt return
-            Dep_Option B a_opt -> Dep_Option_elimT B' a_opt with
-        | Some a => fun b => f (Dep_Option_elim b)
-        | None => fun _ => tt
-      end b_opt.
-  Proof.
-    unfold Dep_Option_elim, Dep_Option_Map; destruct b_opt; reflexivity.
-  Qed.
-
-  (* Concrete values for [a_opt] produce corrolaries of
-     [Dep_Option_Map_elim] with nicer statements. *)
-  Corollary Dep_Option_Map_elim_Some
-  : forall (a : A)
-           (b_opt : Dep_Option B (Some a)),
-      Dep_Option_elim (Dep_Option_Map b_opt) = f (Dep_Option_elim b_opt).
-  Proof.
-    intros; eapply Dep_Option_Map_elim; eauto.
-  Qed.
-
-  Corollary Dep_Option_Map_elim_None
-  : forall (b_opt : Dep_Option B None),
-      Dep_Option_elim (Dep_Option_Map b_opt) = tt.
-  Proof.
-    intros; eapply Dep_Option_Map_elim; eauto.
-  Qed.
-
-  (* [imap] behaves as expected with the [ith_error] lookup
-     function as well, albeit with a more dependently-typed statement. *)
-  Lemma ith_error_imap :
-    forall (n : nat)
-           (As : list A)
-           (il : ilist _ As),
-      Dep_Option_Map (ith_error il n) =
-      ith_error (imap il) n.
-  Proof.
-    induction n; destruct As; simpl; eauto;
-    intros; icons_invert; simpl; auto.
-  Qed.
-
-End ilist_imap.
-
-Section ilist_izip.
-
-  (* Merging two indexed lists together. *)
-
-  Variable A : Type. (* The indexing type. *)
-  Variable B B' D : A -> Type. (* The three types of indexed elements. *)
-  Variable f : forall a, B a -> B' a -> D a.
-
-  (* The function which merges the two sets of elements. *)
-  Fixpoint izip (As : list A)
-           (il : ilist B As) (il' : ilist B' As)
-  : ilist D As :=
-    match As return ilist B As -> ilist B' As -> ilist D As with
-      | a :: As' =>
-        fun il il' =>
-          icons a (f (ilist_hd il) (ilist_hd il'))
-                (izip (ilist_tl il) (ilist_tl il'))
-      | [] => fun il il' => inil D
-    end il il'.
-
-  (* [izip] behaves as expected with the [ith_default] lookup
-     function. *)
-  Lemma ith_default_izip :
-    forall (n : nat)
-           (As : list A)
-           (il : ilist B As)
-           (il' : ilist B' As)
-           (default_A : A)
-           (default_B : B default_A)
-           (default_B' : B' default_A),
-      ith_default _ (f default_B default_B') (izip il il') n =
-      f (ith_default _ default_B il n) (ith_default _ default_B' il' n).
-  Proof.
-    induction n; destruct As; simpl; eauto;
-    intros; icons_invert; simpl; auto.
-  Qed.
-
-  (* Merging two dependent options together. *)
-  Definition Dep_Option_Zip
-             (a_opt : option A)
-             (b_opt : Dep_Option B a_opt)
-             (b'_opt : Dep_Option B' a_opt):
-    Dep_Option D a_opt :=
-    match a_opt return
-          Dep_Option B a_opt -> Dep_Option B' a_opt ->
-          Dep_Option D a_opt with
-      | Some a =>
-        fun b b' =>
-          Dep_Some D a (f (Dep_Option_elim b) (Dep_Option_elim b'))
-      | None => fun _ _ => Dep_None D
-    end b_opt b'_opt.
-
-  (* Projecting the combination of two dependent sums [b_opt] and [b'_opt]
-     is the same as combining the projections of [b_opt] and [b'_opt]. *)
-  Lemma Dep_Option_Zip_elim
-  : forall (a_opt : option A)
-           (b_opt : Dep_Option B a_opt)
-           (b'_opt : Dep_Option B' a_opt),
-      Dep_Option_elim (Dep_Option_Zip b_opt b'_opt) =
-      match a_opt return
-            Dep_Option B a_opt
-            -> Dep_Option B' a_opt
-            -> Dep_Option_elimT D a_opt with
-        | Some a => fun b b' => f (Dep_Option_elim b) (Dep_Option_elim b')
-        | None => fun _ _ => tt
-      end b_opt b'_opt.
-  Proof.
-    unfold Dep_Option_elim, Dep_Option_Zip; destruct b_opt; reflexivity.
-  Qed.
-
-  (* Concrete values for [a_opt] produce corrolaries of
-     [Dep_Option_Zip_elim] with nicer statements. *)
-  Corollary Dep_Option_Zip_elim_Some
-  : forall (a : A)
-           (b_opt : Dep_Option B (Some a))
-           (b'_opt : Dep_Option B' (Some a)),
-      Dep_Option_elim (Dep_Option_Zip b_opt b'_opt) =
-      f (Dep_Option_elim b_opt) (Dep_Option_elim b'_opt).
-  Proof.
-    intros; eapply Dep_Option_Zip_elim; eauto.
-  Qed.
-
-  Corollary Dep_Option_Zip_elim_None
-  : forall (b_opt : Dep_Option B None)
-           (b'_opt : Dep_Option B' None),
-      Dep_Option_elim (Dep_Option_Zip b_opt b'_opt) = tt.
-  Proof.
-    intros; eapply Dep_Option_Zip_elim; eauto.
-  Qed.
-
-  (* [izip] behaves as expected with the [ith_error] lookup
-     function as well, albeit with a more dependently-typed statement. *)
-
-  Lemma ith_error_izip :
-    forall (n : nat)
-           (As : list A)
-           (il : ilist B As)
-           (il' : ilist B' As),
-      ith_error (izip il il') n =
-      Dep_Option_Zip (ith_error il n) (ith_error il' n).
-  Proof.
-    induction n; destruct As; simpl; eauto;
-    intros; icons_invert; simpl; auto.
-  Qed.
-
-End ilist_izip.
-*)
-
 Section i2list2_replace.
 
   (* Replacing an element of an indexed list. *)
@@ -506,30 +196,30 @@ Section i2list2_replace.
   Program Fixpoint replace_2Index2
            (n : nat)
            (As : list A)
-           (Bs : ilist B As)
+           (Bs : ilist2 B As)
            (Cs : i2list2 C Bs)
-           (new_c : Dep_Option_elim_P C (ith_error Bs n))
+           (new_c : Dep_Option_elim_P C (ith2_error Bs n))
            {struct Bs} : i2list2 C Bs :=
     match n return
             i2list2 C Bs
-            -> Dep_Option_elim_P C (ith_error Bs n)
+            -> Dep_Option_elim_P C (ith2_error Bs n)
             -> i2list2 C Bs with
       | 0 => match Bs return
                      i2list2 C Bs
-                     -> Dep_Option_elim_P C (ith_error Bs 0)
+                     -> Dep_Option_elim_P C (ith2_error Bs 0)
                      -> i2list2 C Bs with
-                 | inil =>
+                 | inil2 =>
                    fun il _ => i2nil2 _ _
-                 | icons a b As' Bs' =>
+                 | icons2 a b As' Bs' =>
                    fun Cs' new_c =>
                      i2cons2 _ new_c (i2list2_tl Cs')
                end
       | S n => match Bs return
                      i2list2 C Bs
-                     -> Dep_Option_elim_P C (ith_error Bs (S n))
+                     -> Dep_Option_elim_P C (ith2_error Bs (S n))
                      -> i2list2 C Bs with
-                 | inil => fun il _ => i2nil2 _ _
-                 | icons a As' b Bs' =>
+                 | inil2 => fun il _ => i2nil2 _ _
+                 | icons2 a As' b Bs' =>
                    fun Cs' new_c =>
                      i2cons2 _ (i2list2_hd Cs')
                             (@replace_2Index2 n As' Bs'
@@ -577,15 +267,15 @@ Section i2list2_replace.
   : forall
       (n : nat)
       (As : list A)
-      (Bs : ilist _ As)
+      (Bs : ilist2 _ As)
       (Cs : i2list2 C Bs)
       (n' : nat)
-      (new_c : Dep_Option_elim_P C (ith_error Bs n')),
+      (new_c : Dep_Option_elim_P C (ith2_error Bs n')),
       n <> n'
       -> i2th_error2 (replace_2Index2 n' Cs new_c) n =
          i2th_error2 Cs n.
   Proof.
-    induction n; simpl; destruct Bs; intros; icons_invert;
+    induction n; simpl; destruct Bs; intros; icons2_invert;
     simpl in *; auto;
     destruct n'; simpl; try congruence.
     eapply IHn; congruence.
@@ -595,9 +285,9 @@ Section i2list2_replace.
   : forall
       (n : nat)
       (As : list A)
-      (Bs : ilist _ As)
+      (Bs : ilist2 _ As)
       (Cs : i2list2 C Bs)
-      (new_c : Dep_Option_elim_P C (ith_error Bs n)),
+      (new_c : Dep_Option_elim_P C (ith2_error Bs n)),
       i2th_error2 (replace_2Index2 n Cs new_c) n = new_c.
   Proof.
     induction n; destruct Bs; simpl; auto; intros;
@@ -607,15 +297,15 @@ Section i2list2_replace.
   Program Fixpoint replace_2Index2'
            (n : nat)
            (As : list A)
-           (Bs : ilist B As)
+           (Bs : ilist2 B As)
            (Cs : i2list2 C Bs)
-           (new_c : Dep_Option_elim_P C (ith_error Bs n))
+           (new_c : Dep_Option_elim_P C (ith2_error Bs n))
            {struct Cs} : i2list2 C Bs :=
     match n return
-          Dep_Option_elim_P C (ith_error Bs n)
+          Dep_Option_elim_P C (ith2_error Bs n)
             -> i2list2 C Bs with
       | 0 => match Cs in i2list2 _ Bs return
-                   Dep_Option_elim_P C (ith_error Bs 0)
+                   Dep_Option_elim_P C (ith2_error Bs 0)
                    -> i2list2 C Bs with
                  | i2nil2 Bs =>
                    fun _ => i2nil2 _ Bs
@@ -624,12 +314,12 @@ Section i2list2_replace.
                      i2cons2 Bs' new_c i2l'
                end
       | S n => match Cs in i2list2 _ Bs return
-                     Dep_Option_elim_P C (ith_error Bs (S n))
+                     Dep_Option_elim_P C (ith2_error Bs (S n))
                      -> i2list2 C Bs with
                  | i2nil2 Bs => fun _ => i2nil2 _ Bs
                  | i2cons2 a As' Bs' c i2l' =>
                    fun new_c =>
-                     i2cons2 Bs' c (@replace_2Index2' n As' (ilist_tl Bs') i2l' new_c)
+                     i2cons2 Bs' c (@replace_2Index2' n As' (ilist2_tl Bs') i2l' new_c)
                end
     end new_c.
 
@@ -637,15 +327,15 @@ Section i2list2_replace.
   : forall
       (n : nat)
       (As : list A)
-      (Bs : ilist _ As)
+      (Bs : ilist2 _ As)
       (Cs : i2list2 C Bs)
       (n' : nat)
-      (new_c : Dep_Option_elim_P C (ith_error Bs n')),
+      (new_c : Dep_Option_elim_P C (ith2_error Bs n')),
       n <> n'
       -> i2th_error2' (replace_2Index2' n' Cs new_c) n =
          i2th_error2' Cs n.
   Proof.
-    induction n; simpl; destruct Cs; intros; icons_invert;
+    induction n; simpl; destruct Cs; intros; icons2_invert;
     simpl in *; auto;
     destruct n'; simpl; try congruence.
     unfold replace_2Index2.
@@ -656,9 +346,9 @@ Section i2list2_replace.
   : forall
       (n : nat)
       (As : list A)
-      (Bs : ilist _ As)
+      (Bs : ilist2 _ As)
       (Cs : i2list2 C Bs)
-      (new_c : Dep_Option_elim_P C (ith_error Bs n)),
+      (new_c : Dep_Option_elim_P C (ith2_error Bs n)),
       i2th_error2' (replace_2Index2' n Cs new_c) n = new_c.
   Proof.
     induction n; destruct Cs; simpl; auto; intros;
